CollapsingTowers/TwoLevelRec/LogicalEquiv/Fundamental.lean
@@ -3,10 +3,10 @@ import CollapsingTowers.TwoLevelRec.LogicalEquiv.Compatibility
 -- Γ ⊢ e : τ
 -- ————————————————
 -- Γ ⊧ e ≤𝑙𝑜𝑔 e : τ
-theorem log_rel_typing.fundamental :
+theorem log_approx.fundamental :
   ∀ Γ e τ,
     typing Γ 𝟚 e τ ∅ →
-    log_rel_typing Γ e e τ :=
+    log_approx Γ e e τ :=
   by
   generalize HEq𝕊 : 𝟚 = 𝕊
   generalize HEqφ : ∅ = φ
@@ -14,7 +14,7 @@ theorem log_rel_typing.fundamental :
   revert HEq𝕊 HEqφ
   apply @typing.rec
     (fun Γ 𝕊 e τ φ (H : typing Γ 𝕊 e τ φ) =>
-      𝟚 = 𝕊 → ∅ = φ → log_rel_typing Γ e e τ)
+      𝟚 = 𝕊 → ∅ = φ → log_approx Γ e e τ)
     (fun Γ e τ φ (H : typing_reification Γ e τ φ) => true)
   <;> intros
   <;> (try contradiction)
@@ -66,11 +66,11 @@ theorem log_rel_typing.fundamental :
   case reify => simp
   apply Hτ
 
-lemma log_rel_value.fundamental :
+lemma log_approx_value.fundamental :
   ∀ k v τ,
     value v →
     typing [] 𝟚 v τ ∅ →
-    log_rel_value k v v τ :=
+    log_approx_value k v v τ :=
   by
   intros k v τ Hvalue Hτ
   cases k
@@ -81,7 +81,7 @@ lemma log_rel_value.fundamental :
       cases τ
       case arrow τ𝕒 τ𝕓 φ =>
         cases φ <;> simp at Hwbt
-        simp only [log_rel_value]
+        simp only [log_approx_value]
         constructor; apply Hτ
         constructor; apply Hτ
         simp
@@ -91,22 +91,22 @@ lemma log_rel_value.fundamental :
       simp
     case code => nomatch Hτ
   case succ k =>
-    have ⟨_, _, Hsem_expr⟩ := log_rel_typing.fundamental _ _ _ Hτ
-    simp only [log_rel_expr] at Hsem_expr
-    have ⟨r, Hstep, Hsem_value⟩ := Hsem_expr (k + 1) _ _ (log_rel_env.nil _) 0 (by omega) _ Hvalue (stepn_indexed.refl _)
+    have ⟨_, _, Hsem_expr⟩ := log_approx.fundamental _ _ _ Hτ
+    simp only [log_approx_expr] at Hsem_expr
+    have ⟨r, Hstep, Hsem_value⟩ := Hsem_expr (k + 1) _ _ (log_approx_env.nil _) 0 (by omega) _ Hvalue (stepn_indexed.refl _)
     rw [← stepn.value_impl_termination _ _ Hvalue Hstep] at Hsem_value
     apply Hsem_value
 
-lemma log_rel_env.fundamental :
+lemma log_approx_env.fundamental :
   ∀ k γ Γ,
     typing.subst γ Γ →
-    log_rel_env k γ γ Γ :=
+    log_approx_env k γ γ Γ :=
   by
   intros k γ Γ HτΓ
   induction HτΓ
-  case nil => apply log_rel_env.nil
+  case nil => apply log_approx_env.nil
   case cons v γ τ Γ Hvalue Hτ _ IH =>
-    apply log_rel_env.cons
-    . apply log_rel_value.fundamental
+    apply log_approx_env.cons
+    . apply log_approx_value.fundamental
       apply Hvalue; apply Hτ
     . apply IH
