CollapsingTowers/TwoLevelRec/LogicalEquiv/Soundness.lean
@@ -1,11 +1,11 @@
 import CollapsingTowers.TwoLevelRec.LogicalEquiv.Fundamental
 import CollapsingTowers.TwoLevelRec.CtxEquiv.Defs
 
-lemma log_rel_typing.congruence_under_ObsCtx𝔹 :
+lemma log_approx.congruence_under_ObsCtx𝔹 :
   ∀ Δ Γ τδ τγ B e₀ e₁,
-    log_rel_typing Δ e₀ e₁ τδ →
+    log_approx Δ e₀ e₁ τδ →
     ObsCtx𝔹 Δ τδ B Γ τγ →
-    log_rel_typing Γ B⟦e₀⟧ B⟦e₁⟧ τγ :=
+    log_approx Γ B⟦e₀⟧ B⟦e₁⟧ τγ :=
   by
   intros Δ Γ τδ τγ B e₀ e₁ Hsem HB
   have ⟨Hτ₀, Hτ₁, Hsem_expr⟩ := Hsem
@@ -22,10 +22,10 @@ lemma log_rel_typing.congruence_under_ObsCtx𝔹 :
   case appl₁ Harg =>
     apply compatibility.app₁
     . apply Hsem
-    . apply log_rel_typing.fundamental _ _ _ Harg
+    . apply log_approx.fundamental _ _ _ Harg
   case appr₁ Hf =>
     apply compatibility.app₁
-    . apply log_rel_typing.fundamental _ _ _ Hf
+    . apply log_approx.fundamental _ _ _ Hf
     . apply Hsem
   case letsl τ𝕒 τ𝕓 Hclosed He =>
     apply compatibility.lets
@@ -34,14 +34,14 @@ lemma log_rel_typing.congruence_under_ObsCtx𝔹 :
     . apply Hclosed
     . apply Hclosed
     . apply Hsem
-    . apply log_rel_typing.fundamental _ _ _ He
+    . apply log_approx.fundamental _ _ _ He
   case letsr τ𝕒 τ𝕓 Hb =>
     apply compatibility.lets
     . have ⟨Hwbt, _⟩ := typing.wbt_pure_at_dyn _ _ _ _ Hb
       apply Hwbt
     . rw [← closed.under_closing]; apply typing.closed_at_env _ _ _ _ _ Hτ₀
     . rw [← closed.under_closing]; apply typing.closed_at_env _ _ _ _ _ Hτ₁
-    . apply log_rel_typing.fundamental _ _ _ Hb
+    . apply log_approx.fundamental _ _ _ Hb
     . rw [identity.opening_closing, identity.opening_closing]
       apply Hsem
       apply typing.regular; apply Hτ₁
@@ -54,26 +54,26 @@ lemma log_rel_typing.congruence_under_ObsCtx𝔹 :
 -- Γ ⊢ C⟦Δ ⊢ τδ⟧ : τγ
 -- ————————————————————————
 -- Γ ⊧ C⟦e₀⟧ ≤𝑙𝑜𝑔 C⟦e₁⟧ : τγ
-lemma log_rel_typing.congruence_under_ObsCtxℂ :
+lemma log_approx.congruence_under_ObsCtxℂ :
   ∀ Δ Γ τδ τγ C e₀ e₁,
-    log_rel_typing Δ e₀ e₁ τδ →
+    log_approx Δ e₀ e₁ τδ →
     ObsCtxℂ Δ τδ C Γ τγ →
-    log_rel_typing Γ C⟦e₀⟧ C⟦e₁⟧ τγ :=
+    log_approx Γ C⟦e₀⟧ C⟦e₁⟧ τγ :=
   by
   intros Δ Γ τδ τγ C e₀ e₁ Hsem HC
   induction HC generalizing e₀ e₁
   case hole => apply Hsem
   case cons𝔹 HB IH =>
     apply IH
-    apply log_rel_typing.congruence_under_ObsCtx𝔹
+    apply log_approx.congruence_under_ObsCtx𝔹
     apply Hsem; apply HB
 
 -- Γ ⊧ e₀ ≤𝑙𝑜𝑔 e₁ : τ
 -- ——————————————————
 -- Γ ⊢ e₀ ≤𝑐𝑡𝑥 e₁ : τ
-theorem log_rel_typing.soundness :
+theorem log_approx.soundness :
   ∀ Γ τ e₀ e₁,
-    log_rel_typing Γ e₀ e₁ τ →
+    log_approx Γ e₀ e₁ τ →
     ctx_approx Γ e₀ e₁ τ :=
   by
   intros Γ τ e₀ e₁ Hsem Hτ₀ Hτ₁ C
@@ -85,13 +85,13 @@ theorem log_rel_typing.soundness :
     have ⟨k, Hstep₀⟩ := stepn_impl_stepn_indexed _ _ Hstep₀
     rw [← HEqΔ] at Hsem
     have ⟨Hwf₀, Hwf₁, Hsem_expr⟩ := Hsem
-    simp only [log_rel_expr] at Hsem_expr
-    have ⟨v₁, Hstep₁, Hsem_value⟩ := Hsem_expr (k + 1) _ _ (log_rel_env.nil _) k (by omega) _ Hvalue₀ Hstep₀
-    have ⟨_, Hvalue₁⟩ := log_rel_value.syntactic.value _ _ _ _ Hsem_value
+    simp only [log_approx_expr] at Hsem_expr
+    have ⟨v₁, Hstep₁, Hsem_value⟩ := Hsem_expr (k + 1) _ _ (log_approx_env.nil _) k (by omega) _ Hvalue₀ Hstep₀
+    have ⟨_, Hvalue₁⟩ := log_approx_value.syntactic.value _ _ _ _ Hsem_value
     exists v₁
   case cons𝔹 C B HC HB IH =>
     apply IH
-    apply log_rel_typing.congruence_under_ObsCtx𝔹
+    apply log_approx.congruence_under_ObsCtx𝔹
     apply Hsem; apply HB
     apply typing.congruence_under_ObsCtx𝔹; apply Hτ₀; apply HB
     apply typing.congruence_under_ObsCtx𝔹; apply Hτ₁; apply HB
