CollapsingTowers/TwoLevelRec/LogicalEquiv/Transitive.lean
@@ -1,10 +1,10 @@
 import CollapsingTowers.TwoLevelRec.LogicalEquiv.Fundamental
 
 mutual
-lemma log_rel_value.trans (k : Nat) (v₀ v₁ v₂ : Expr) (τ : Ty) :
-    log_rel_value k v₀ v₁ τ →
-    (∀ k, log_rel_value k v₁ v₂ τ) →
-    log_rel_value k v₀ v₂ τ :=
+lemma log_approx_value.trans (k : Nat) (v₀ v₁ v₂ : Expr) (τ : Ty) :
+    log_approx_value k v₀ v₁ τ →
+    (∀ k, log_approx_value k v₁ v₂ τ) →
+    log_approx_value k v₀ v₂ τ :=
     match τ with
     | .nat =>
       by
@@ -22,21 +22,21 @@ lemma log_rel_value.trans (k : Nat) (v₀ v₁ v₂ : Expr) (τ : Ty) :
       case lam e₁ =>
       cases v₂ <;> try simp at Hsem_value₁
       case lam e₂ =>
-      cases φ <;> simp only [log_rel_value] at Hsem_value₀ Hsem_value₁ <;> try contradiction
-      simp only [log_rel_value]
+      cases φ <;> simp only [log_approx_value] at Hsem_value₀ Hsem_value₁ <;> try contradiction
+      simp only [log_approx_value]
       have ⟨Hτ₀, Hτ₁, Hsem_expr₀⟩ := Hsem_value₀
       have ⟨Hτ₁, Hτ₂, _⟩ := Hsem_value₁ 0
       constructor; apply Hτ₀
       constructor; apply Hτ₂
       intros j Hindexj argv₀ argv₁ Hsem_value_arg₀
-      have ⟨HvalueArg₀, HvalueArg₁⟩ := log_rel_value.syntactic.value _ _ _ _ Hsem_value_arg₀
-      have ⟨HτArg₀, HτArg₁⟩ := log_rel_value.syntactic.typing _ _ _ _ Hsem_value_arg₀
-      apply log_rel_expr.trans; apply Hsem_expr₀
+      have ⟨HvalueArg₀, HvalueArg₁⟩ := log_approx_value.syntactic.value _ _ _ _ Hsem_value_arg₀
+      have ⟨HτArg₀, HτArg₁⟩ := log_approx_value.syntactic.typing _ _ _ _ Hsem_value_arg₀
+      apply log_approx_expr.trans; apply Hsem_expr₀
       apply Hindexj; apply Hsem_value_arg₀
       intros k
       have ⟨Hτ₁, Hτ₂, Hsem_expr₁⟩ := Hsem_value₁ k
       apply Hsem_expr₁; rfl
-      apply log_rel_value.fundamental
+      apply log_approx_value.fundamental
       apply HvalueArg₁; apply HτArg₁
     | .fragment _ => by simp
     | .rep _ => by simp
@@ -44,32 +44,32 @@ lemma log_rel_value.trans (k : Nat) (v₀ v₁ v₂ : Expr) (τ : Ty) :
 termination_by (τ, k)
 decreasing_by apply Prod.Lex.left; simp; omega
 
-lemma log_rel_expr.trans :
+lemma log_approx_expr.trans :
   ∀ k e₀ e₁ e₂ τ,
-    log_rel_expr k e₀ e₁ τ →
-    (∀ k, log_rel_expr k e₁ e₂ τ) →
-    log_rel_expr k e₀ e₂ τ :=
+    log_approx_expr k e₀ e₁ τ →
+    (∀ k, log_approx_expr k e₁ e₂ τ) →
+    log_approx_expr k e₀ e₂ τ :=
   by
   intros k e₀ e₁ e₂ τ Hsem_expr₀ Hsem_expr₁
   cases k
   case zero => simp
   case succ k =>
-    simp only [log_rel_expr] at Hsem_expr₀ Hsem_expr₁
-    simp only [log_rel_expr]
+    simp only [log_approx_expr] at Hsem_expr₀ Hsem_expr₁
+    simp only [log_approx_expr]
     intros i₀ Hindexi₀ v₀ Hvalue₀ Hstep₀
     have ⟨v₁, Hstep₁, Hsem_value₀⟩ := Hsem_expr₀ _ Hindexi₀ _ Hvalue₀ Hstep₀
-    have ⟨Hvalue₀, Hvalue₁⟩ := log_rel_value.syntactic.value _ _ _ _ Hsem_value₀
+    have ⟨Hvalue₀, Hvalue₁⟩ := log_approx_value.syntactic.value _ _ _ _ Hsem_value₀
     have ⟨i₁, Hstep₁⟩ := stepn_impl_stepn_indexed _ _ Hstep₁
     have ⟨v₂, Hstep₂, Hsem_value₁⟩ := Hsem_expr₁ (i₁ + 1) i₁ (by omega) _ Hvalue₁ Hstep₁
-    have ⟨Hvalue₁, Hvalue₂⟩ := log_rel_value.syntactic.value _ _ _ _ Hsem_value₁
+    have ⟨Hvalue₁, Hvalue₂⟩ := log_approx_value.syntactic.value _ _ _ _ Hsem_value₁
     exists v₂
     constructor; apply Hstep₂
-    apply log_rel_value.trans; apply Hsem_value₀
+    apply log_approx_value.trans; apply Hsem_value₀
     intros k
     have ⟨v₃, Hstep₃, Hsem_value₂⟩ := Hsem_expr₁ (k + i₁ + 1) i₁ (by omega) _ Hvalue₁ Hstep₁
-    have ⟨Hvalue₁, Hvalue₃⟩ := log_rel_value.syntactic.value _ _ _ _ Hsem_value₂
+    have ⟨Hvalue₁, Hvalue₃⟩ := log_approx_value.syntactic.value _ _ _ _ Hsem_value₂
     rw [stepn.unique_normal_forms _ _ _ Hstep₂ Hstep₃ Hvalue₂ Hvalue₃]
-    apply log_rel_value.antimono
+    apply log_approx_value.antimono
     apply Hsem_value₂; omega
 
 termination_by k _ _ _ τ => (τ, k + 1)
@@ -80,11 +80,11 @@ end
 -- Γ ⊧ e₁ ≤𝑙𝑜𝑔 e₂ : τ
 -- ——————————————————
 -- Γ ⊧ e₀ ≤𝑙𝑜𝑔 e₂ : τ
-theorem log_rel_typing.trans :
+theorem log_approx.trans :
   ∀ Γ e₀ e₁ e₂ τ,
-    log_rel_typing Γ e₀ e₁ τ →
-    log_rel_typing Γ e₁ e₂ τ →
-    log_rel_typing Γ e₀ e₂ τ :=
+    log_approx Γ e₀ e₁ τ →
+    log_approx Γ e₁ e₂ τ →
+    log_approx Γ e₀ e₂ τ :=
   by
   intros Γ e₀ e₁ e₂ τ H₀ H₁
   have ⟨Hτ₀, Hτ₁, H₀⟩ := H₀
@@ -92,9 +92,9 @@ theorem log_rel_typing.trans :
   constructor; apply Hτ₀
   constructor; apply Hτ₂
   intros k γ₀ γ₁ HsemΓ
-  have ⟨HτΓ₀, HτΓ₁⟩ := log_rel_env.syntactic.typing _ _ _ _ HsemΓ
-  apply log_rel_expr.trans
+  have ⟨HτΓ₀, HτΓ₁⟩ := log_approx_env.syntactic.typing _ _ _ _ HsemΓ
+  apply log_approx_expr.trans
   apply H₀; apply HsemΓ
   intro k; apply H₁
-  apply log_rel_env.fundamental
+  apply log_approx_env.fundamental
   apply HτΓ₁
